Fix proofs in targetProps, change backend_correct
The encoder correctness (backend_correct) proofs are not yet updated.

The changes required are that more things don't change during execution
of asm instructions (plus interference):
  - the code being executed is not changed in memory during execution, and,
  - equal projections implies equal pcs and equal memories (under the
    domain) (these two were only available alongside the rest of the
    target_state_rel conditions, not individually).

compiler/backend/semantics/targetSemScript.sml
@@ -38,9 +38,9 @@ val apply_oracle_def = Define `
 
 val encoded_bytes_in_mem_def = Define`
   encoded_bytes_in_mem c pc m md ⇔
-    ∃i k. k * c.code_alignment < LENGTH (c.encode i) ∧
+    ∃i k. k (** c.code_alignment*) < LENGTH (c.encode i) ∧
       bytes_in_memory pc
-        (DROP (k * c.code_alignment) (c.encode i))
+        (DROP (k (** c.code_alignment*)) (c.encode i))
         m md`;
 
 val evaluate_def = Define `
